Got rid of all uses of heterogenous equality from SF files
as suggested by Nik

examples/unit-tests/sf-lists.fst
@@ -12,8 +12,6 @@ type ilist =
   | Nil : ilist
   | Cons : int -> ilist -> ilist
 
-type nat = i:int{i >= 0}
-
 val length : ilist -> Tot nat
 let rec length l =
   match l with
@@ -34,25 +32,25 @@ let rec app l1 l2 =
 
 val test_app1 : unit -> Fact unit
       (ensures (app (Cons 1 (Cons 2 (Cons 3 Nil))) (Cons 4 (Cons 5 Nil))
-                == (Cons 1 (Cons 2 (Cons 3 (Cons 4 (Cons 5 Nil)))))))
+                = (Cons 1 (Cons 2 (Cons 3 (Cons 4 (Cons 5 Nil)))))))
 let test_app1 () = ()
 
 val test_app2 : unit -> Fact unit
       (ensures (app Nil (Cons 4 (Cons 5 Nil))
-                == (Cons 4 (Cons 5 Nil))))
+                = (Cons 4 (Cons 5 Nil))))
 let test_app2 () = ()
 
 val test_app3 : unit -> Fact unit
       (ensures (app (Cons 1 (Cons 2 (Cons 3 Nil))) Nil)
-                == (Cons 1 (Cons 2 (Cons 3 Nil))))
+                = (Cons 1 (Cons 2 (Cons 3 Nil))))
 let test_app3 () = ()
 
 val nil_app : l:ilist -> Fact unit
-                              (ensures (app Nil l == l))
+                              (ensures (app Nil l = l))
 let nil_app l = ()
 
 val app_nil : l:ilist -> Fact unit
-                              (ensures (app l Nil == l))
+                              (ensures (app l Nil = l))
 let rec app_nil l =
   match l with
   | Nil -> ()
@@ -63,7 +61,7 @@ let hd l =
   match l with
   | Cons h t -> h
 
-(* In SF they have tl Nil == nil, but we do better below *)
+(* In SF they have tl Nil = nil, but we do better below *)
 
 val tl_strange : l:ilist -> Tot ilist
 let tl_strange l =
@@ -72,11 +70,11 @@ let tl_strange l =
   | Cons h t -> t
 
 val tl_strange_length_pred : l:ilist{l =!= Nil} -> Fact unit
-      (ensures ((length l) - 1 == length (tl_strange l)))
+      (ensures ((length l) - 1 = length (tl_strange l)))
 let tl_strange_length_pred l = ()
 
 val tl_strange_length_pred_equiv : l:ilist{is_Cons l} -> Fact unit
-      (ensures ((length l) - 1 == length (tl_strange l)))
+      (ensures ((length l) - 1 = length (tl_strange l)))
 let tl_strange_length_pred_equiv l = ()
 
 val tl : l:ilist{l =!= Nil} -> Tot ilist
@@ -85,18 +83,18 @@ let tl l =
   | Cons h t -> t
 
 val tl_length_pred : l:ilist{l =!= Nil} -> Fact unit
-      (ensures ((length l) - 1 == length (tl l)))
+      (ensures ((length l) - 1 = length (tl l)))
 let tl_length_pred l = ()
 
 val app_assoc : l1 : ilist -> l2 : ilist -> l3 : ilist -> Fact unit
-      (ensures (app (app l1 l2) l3) == app l1 (app l2 l3))
+      (ensures (app (app l1 l2) l3) = app l1 (app l2 l3))
 let rec app_assoc l1 l2 l3 =
   match l1 with
   | Nil -> ()
   | Cons h t -> app_assoc t l2 l3
 
 val app_length : l1 : ilist -> l2 : ilist -> Fact unit
-      (ensures (length (app l1 l2) == (length l1) + (length l2)))
+      (ensures (length (app l1 l2) = (length l1) + (length l2)))
 let rec app_length l1 l2 =
   match l1 with
   | Nil -> ()
@@ -115,41 +113,41 @@ let rec rev l =
   | Cons h t -> snoc (rev t) h
 
 val length_snoc : n : int -> l : ilist -> Fact unit
-      (ensures (length (snoc l n) == length l + 1))
+      (ensures (length (snoc l n) = length l + 1))
 let rec length_snoc n l =
   match l with
   | Nil -> ()
   | Cons h t -> length_snoc n t
 
 val rev_length : l : ilist -> Fact unit
-      (ensures (length (rev l) == length l))
+      (ensures (length (rev l) = length l))
 let rec rev_length l =
   match l with
   | Nil -> ()
   | Cons h t -> length_snoc h (rev t); rev_length t
 
 val foo1 : n:int -> l : ilist -> Pure unit
-      (requires (repeat n 0 == l))
-      (ensures \r => length l == 0)
+      (requires (repeat n 0 = l))
+      (ensures \r => length l = 0)
 let foo1 n l = ()
 
 val foo2 : n : nat -> m : nat -> l : ilist -> Pure unit
-      (requires (repeat n m == l))
-      (ensures \r => length l == m)
+      (requires (repeat n m = l))
+      (ensures \r => length l = m)
 let rec foo2 n m l =
   match m with
   | 0 -> () 
   | _ -> foo2 n (m-1) (repeat n (m-1))
 
-val foo3 : l : ilist -> n : int -> m : int -> Pure unit
-      (requires (length l == m))
-      (ensures \r => (length (snoc l n) == m+1))
+val foo3 : l : ilist -> n : int -> m : nat -> Pure unit
+      (requires (length l = m))
+      (ensures \r => (length (snoc l n) = m+1))
 let rec foo3 l n m =
   match l with
   | Nil -> ()
   | Cons h t -> foo3 t n (length t)
 
 val foo4 : n : int -> l1 : ilist -> l2 : ilist -> Pure unit
-      (requires (snoc l1 n == l2))
+      (requires (snoc l1 n = l2))
       (ensures \r => 0 < length l2)
 let foo4 n l1 l2 = ()
