examples/unit-tests/sf-basic.fst
@@ -27,7 +27,7 @@ let next_weekday d =
   | Sunday    -> Monday
 
 val test_next_weekday : unit -> Fact unit
-      (ensures ((next_weekday (next_weekday Saturday)) == Tuesday))
+      (ensures ((next_weekday (next_weekday Saturday)) = Tuesday))
 let test_next_weekday () = ()
 
 (* Booleans *)
@@ -59,19 +59,19 @@ let orb b1 b2 =
   | MFalse -> b2
 
 val test_orb1 : unit -> Fact unit
-      (ensures ((orb MTrue MFalse) == MTrue))
+      (ensures ((orb MTrue MFalse) = MTrue))
 let test_orb1 () = ()
 
 val test_orb2 : unit -> Fact unit
-      (ensures ((orb MFalse MFalse) == MFalse))
+      (ensures ((orb MFalse MFalse) = MFalse))
 let test_orb2 () = ()
 
 val test_orb3 : unit -> Fact unit
-      (ensures ((orb MFalse MTrue) == MTrue))
+      (ensures ((orb MFalse MTrue) = MTrue))
 let test_orb3 () = ()
 
 val test_orb4 : unit -> Fact unit
-      (ensures ((orb MTrue MTrue) == MTrue))
+      (ensures ((orb MTrue MTrue) = MTrue))
 let test_orb4 () = ()
 
 (* Numbers *)
@@ -104,11 +104,11 @@ val oddb : nat -> Tot mbool
 let oddb n = negb (evenb n)
 
 val test_oddb1 : unit -> Fact unit
-      (ensures ((oddb (S O)) == MTrue))
+      (ensures ((oddb (S O)) = MTrue))
 let test_oddb1 () = ()
 
 val test_oddb2 : unit -> Fact unit
-      (ensures (oddb (S (S (S (S O)))) == MFalse))
+      (ensures (oddb (S (S (S (S O)))) = MFalse))
 let test_oddb2 () = ()
 
 val plus : nat -> nat -> Tot nat
@@ -125,7 +125,7 @@ let rec mult n m =
 
 val test_mult1 : unit -> Fact unit
       (ensures (mult (S (S (S O))) (S (S (S O))))
-                == (S (S (S (S (S (S (S (S (S O))))))))))
+                = (S (S (S (S (S (S (S (S (S O))))))))))
 let test_mult1 () = ()
 
 val minus : nat -> nat -> Tot nat
@@ -150,53 +150,53 @@ let rec ble_nat n m =
   | S n', S m' -> ble_nat n' m'
 
 val test_ble_nat1 : unit -> Fact unit
-      (ensures (ble_nat (S (S O)) (S (S O)) == MTrue))
+      (ensures (ble_nat (S (S O)) (S (S O)) = MTrue))
 let test_ble_nat1 () = ()
 
 val test_ble_nat2 : unit -> Fact unit
-      (ensures (ble_nat (S (S O)) (S (S (S (S O)))) == MTrue))
+      (ensures (ble_nat (S (S O)) (S (S (S (S O)))) = MTrue))
 let test_ble_nat2 () = ()
 
 val test_ble_nat3 : unit -> Fact unit
-      (ensures (ble_nat (S (S (S (S O)))) (S (S O)) == MFalse))
+      (ensures (ble_nat (S (S (S (S O)))) (S (S O)) = MFalse))
 let test_ble_nat3 () = ()
 
 (* Proof by Simplification *)
 
 val plus_O_n : n : nat -> Fact unit
-      (ensures (plus O n == n))
+      (ensures (plus O n = n))
 let plus_O_n n = ()
 
 (* Proof by Rewriting *)
 
 val plus_id_example : n : nat -> m : nat -> Pure unit
-      (requires (n == m))
-      (ensures \r => (plus n n == plus m m))
+      (requires (n = m))
+      (ensures \r => (plus n n = plus m m))
 let plus_id_example n m = ()
 
 val mult_0_plus : n : nat -> m : nat -> Fact unit
-      (ensures ((mult (plus O n) m) == mult n m))
+      (ensures ((mult (plus O n) m) = mult n m))
 let mult_0_plus n m = ()
 
 (* Proof by Case Analysis *)
 val plus_1_neq_0 : n : nat -> Fact unit
-      (ensures (beq_nat (plus n (S O)) O == MFalse))
+      (ensures (beq_nat (plus n (S O)) O = MFalse))
 let plus_1_neq_0 n = ()
 
 val negb_involutive : b : mbool -> Fact unit
-      (ensures (negb (negb b) == b))
+      (ensures (negb (negb b) = b))
 let negb_involutive b = ()
 
 (* Proof by Induction (Induction.v) *)
 val plus_0_r : n : nat -> Fact unit
-      (ensures (plus n O == n))
+      (ensures (plus n O = n))
 let rec plus_0_r n =
   match n with
   | O -> ()
   | S n' -> plus_0_r n'
 
 val plus_n_Sm : n : nat -> m : nat -> Fact unit
-    (ensures (S (plus n m) == plus n (S m)))
+    (ensures (S (plus n m) = plus n (S m)))
 let rec plus_n_Sm n m =
   match n with
   | O -> ()
@@ -204,7 +204,7 @@ let rec plus_n_Sm n m =
 
 (* this one uses previous lemma -- needs to be explicit it seems *)
 val plus_comm : n : nat -> m : nat -> Fact unit
-      (ensures (plus n m == plus m n))
+      (ensures (plus n m = plus m n))
 let rec plus_comm n m =
   match n with
   | O -> plus_0_r m
@@ -212,5 +212,5 @@ let rec plus_comm n m =
 
 (* this one uses previous lemma -- needs to be explicit it seems *)
 val plus_rearrange : n : nat -> m : nat -> p : nat -> q : nat -> Fact unit
-      (ensures (plus (plus n m) (plus p q) == plus (plus m n) (plus p q)))
+      (ensures (plus (plus n m) (plus p q) = plus (plus m n) (plus p q)))
 let plus_rearrange n m p q = plus_comm n m
